theories/Object.v
@@ -14,32 +14,3 @@ Arguments OP {_}.
 Arguments δ {_}.
 
 Class Object (Π : Type) (Ω : Type) `{EqDecision Ω} := type : Ω → object_type Π.
-
-Instance augmentation_Object (Ω Ω' Π : Type) `{Object Π Ω, Object Π Ω'} : Object Π (Ω + Ω') :=
-  λ obj,
-    match obj with
-    | inl ω => type ω
-    | inr ω => type ω
-    end.
-
-Instance dsig_Object (Ω Π : Type) (P : Ω → Prop) `{∀ x, Decision (P x), Object Π Ω} : Object Π (dsig P).
-Proof.
-  unfold Object. intros [ω _]. exact (type ω).
-Defined.
-
-Variant sing {Ω} (ω : Ω) := Sing.
-
-Instance sing_eq_dec {Ω} (ω : Ω) : EqDecision (sing ω).
-Proof. solve_decision. Defined.
-
-Instance sing_object `{Object Π Ω} (ω : Ω) : Object Π (sing ω).
-Proof.
-  unfold Object. intros obj. destruct obj. exact (type ω).
-Defined.
-
-Definition singleton {A : Type} (x : A) : sig (eq x) := exist (eq x) x (eq_refl x).
-
-Instance singleton_object {Ω} Π (ω : Ω) `{Object Π Ω} : Object Π (sig (eq ω)).
-Proof.
-  unfold Object. intros [? ?]. exact (type ω).
-Defined.
